\subsection*{a)}

\begin{enumerate}
	%\item $\left( \sum_{i=1}^n |x_i|^p \right)^{1/p} = 1 = \left( \sum_{i=1}^n |y_i|^q \right)^{1/q}$
  \item $x_i y_i \leq \frac{x_i^p}{p} + \frac{y_i^q}{q}$ Desigualdad de Young
  \item $|x_i y_i| \leq \frac{|x_i|^p}{p} + \frac{|y_i|^q}{q}$
  \item $\sum_{i=1}^n |x_i y_i| \leq \sum_{i=1}^n \left( \frac{|x_i|^p}{p} + \frac{|y_i|^q}{q} \right) = \sum_{i=1}^n \frac{|x_i|^p}{p} + \sum_{i=1}^n \frac{|y_i|^q}{q} = \frac{1}{p} \sum_{i=1}^n |x_i|^p + \frac{1}{q} \sum_{i=1}^n |y_i|^q$
	\item $\sum_{i=1}^n |x_i|^p = 1 = \sum_{i=1}^n |y_i|^q \to \frac{1}{p} \sum_{i=1}^n |x_i|^p + \frac{1}{q} \sum_{i=1}^n |y_i|^q = \frac{1}{p} + \frac{1}{q} = 1$
	\item $\sum_{i=1}^n |x_i|^p = 1 = \sum_{i=1}^n |y_i|^q \to \left( \sum_{i=1}^n |x_i|^p \right)^{1/p} = 1 = \left( \sum_{i=1}^n |y_i|^q \right)^{1/q}$
  \item $\sum_{i=1}^n |x_i|^p = 1 = \sum_{i=1}^n |y_i|^q \to \sum_{i=1}^n |x_i y_i| \leq 1 = \left( \sum_{i=1}^n |x_i|^p \right)^{1/p} \left( \sum_{i=1}^n |y_i|^q \right)^{1/q}$
  \item $||u||_p = 1 = ||v||_p \to u,v$ satisfacen H\"{o}lder
  \item Suponer $u,v$ satisfacen $\sum_{i=1}^n |x_i y_i| \leq \left( \sum_{i=1}^n |x_i|^p \right)^{1/p} \left( \sum_{i=1}^n |y_i|^q \right)^{1/q}$
  \item Sean $\alpha, \beta \in R$
  \item $\sum_{i=1}^n | (\alpha x_i) (\beta y_i) | = \sum_{i=1}^n  |\alpha \beta||x_i y_i| = |\alpha \beta| \sum_{i=1}^n |x_i y_i| \leq |\alpha \beta| \left( \sum_{i=1}^n |x_i|^p \right)^{1/p} \left( \sum_{i=1}^n |y_i|^q \right)^{1/q}$
  \item $|\alpha \beta| = |\alpha| |\beta| = |\alpha|^{p/p} |\beta|^{q/q}$
  \item $|\alpha \beta| \left( \sum_{i=1}^n |x_i|^p \right)^{1/p} \left( \sum_{i=1}^n |y_i|^q \right)^{1/q} = |\alpha|^{p/p} |\beta|^{q/q} \left( \sum_{i=1}^n |x_i|^p \right)^{1/p} \left( \sum_{i=1}^n |y_i|^q \right)^{1/q} = \left( \sum_{i=1}^n |\alpha x_i|^p \right)^{1/p} \left( \sum_{i=1}^n |\beta y_i|^q \right)^{1/q}$
  \item $u,v$ satisfacen H\"{o}lder $\to \forall_{\alpha, \beta \in R} \quad \alpha u, \beta v$ satisfacen H\"{o}lder 
\end{enumerate}
