\subsection*{b)}

\begin{enumerate}
	\item $u=0 \; \wedge \; v=0 \to \left( \sum_{i=1}^n |x_i + y_i|^p \right)^{1/p} = 0 \leq \left( \sum_{i=1}^n |x_i|^p \right)^{1/p} + \left( \sum_{i=1}^n |y_i|^p \right)^{1/p} = 0 + 0 = 0$ 
	\item Sean $u \neq 0 \; \wedge \; v \neq 0$
	\item $\forall_{a,b \in R} \quad |a + b| \leq |a| + |b|$
	\item $|x_i + y_i| \leq |x_i| + |y_i|$
	\item $\sum_{i=1}^n |x_i + y_i| \leq \sum_{i=1}^n \left( |x_i| + |y_i| \right) = \sum_{i=1}^n |x_i| + \sum_{i=1}^n |y_i|$
	\item $p = 1 \to ||u||_p = \sum_{i=1}^n |x_i| \;  \wedge \; ||v||_p = \sum_{i=1}^n |y_i| \;  \wedge \; ||u + v||_p = \sum_{i=1}^n |x_i + y_i|$
	\item $p = 1 \to ||u + v||_p \leq ||u||_p + ||v||_p$
	\item Sea $p > 1$

	\item $\sum_{i=1}^n |x_i + y_i| \leq \sum_{i=1}^n \left( |x_i| + |y_i| \right) \to \sum_{i=1}^n |x_i + y_i|^p \leq \sum_{i=1}^n \left( |x_i| + |y_i| \right)^p \to \left( \sum_{i=1}^n |x_i + y_i|^p \right)^{1/p} \leq \left( \sum_{i=1}^n \left( |x_i| + |y_i| \right)^p \right)^{1/p}$
	\item $(|x_i| + |y_i|)^p = (|x_i| + |y_i|) (|x_i| + |y_i|)^{p-1} = |x_i| (|x_i| + |y_i|)^{p-1} + |y_i| (|x_i| + |y_i|)^{p-1}$
	\item $\sum_{i=1}^n (|x_i| + |y_i|)^p = \sum_{i=1}^n |x_i| (|x_i| + |y_i|)^{p-1} + \sum_{i=1}^n |y_i| (|x_i| + |y_i|)^{p-1} $
	\item $(|x_i| + |y_i|)^{p-1} \geq 0$
	\item H\"{o}lder
	\begin{enumerate}
		\item $\sum_{i=1}^n |x_i| (|x_i| + |y_i|)^{p-1} \leq \left( \sum_{i=1}^n |x_i|^p \right)^{1/p} \left( \sum_{i=1}^n \left[ (|x_i| + |y_i|)^{p-1} \right]^q \right)^{1/q}$
		\item $\sum_{i=1}^n |y_i| (|x_i| + |y_i|)^{p-1} \leq \left( \sum_{i=1}^n |y_i|^p \right)^{1/p} \left( \sum_{i=1}^n \left[ (|x_i| + |y_i|)^{p-1} \right]^q \right)^{1/q}$
	\end{enumerate}
	\item $\sum_{i=1}^n |x_i| (|x_i| + |y_i|)^{p-1} + \sum_{i=1}^n |y_i| (|x_i| + |y_i|)^{p-1} \leq \left[ \left( \sum_{i=1}^n |x_i|^p \right)^{1/p} + \left( \sum_{i=1}^n |y_i|^p \right)^{1/p} \right] \left( \sum_{i=1}^n (|x_i| + |y_i|)^{(p-1)q} \right)^{1/q}$
	\item $\sum_{i=1}^n (|x_i| + |y_i|)^p \leq \left[ \left( \sum_{i=1}^n |x_i|^p \right)^{1/p} + \left( \sum_{i=1}^n |y_i|^p \right)^{1/p} \right] \left( \sum_{i=1}^n (|x_i| + |y_i|)^{(p-1)q} \right)^{1/q}$
	\item $\frac{1}{p} + \frac{1}{q} = 1 \to \frac{q+p}{pq} = 1 \to q+p = pq \to p = pq - q \to p = (p-1)q$
	\item $\sum_{i=1}^n (|x_i| + |y_i|)^p \leq \left[ \left( \sum_{i=1}^n |x_i|^p \right)^{1/p} + \left( \sum_{i=1}^n |y_i|^p \right)^{1/p} \right] \left( \sum_{i=1}^n (|x_i| + |y_i|)^p \right)^{1/q}$
	\item $u \neq 0 \; \wedge \; v \neq 0 \to \left( \sum_{i=1}^n (|x_i| + |y_i|)^p \right)^{1/q} \neq 0$
	\item $\frac{\sum_{i=1}^n (|x_i| + |y_i|)^p}{\left( \sum_{i=1}^n (|x_i| + |y_i|)^p \right)^{1/q}} \leq \left( \sum_{i=1}^n |x_i|^p \right)^{1/p} + \left( \sum_{i=1}^n |y_i|^p \right)^{1/p} $
	\item $\frac{1}{p} + \frac{1}{q} = 1 \to \frac{1}{p} = 1 - \frac{1}{q}$
	\item $\frac{\sum_{i=1}^n (|x_i| + |y_i|)^p}{\left( \sum_{i=1}^n (|x_i| + |y_i|)^p \right)^{1/q}} = \left( \sum_{i=1}^n (|x_i| + |y_i|)^p \right)^{1-\frac{1}{q}} = \left( \sum_{i=1}^n (|x_i| + |y_i|)^p \right)^{\frac{1}{p}}$
	\item $ \left( \sum_{i=1}^n (|x_i + y_i|)^p \right)^{\frac{1}{p}} \leq \left( \sum_{i=1}^n (|x_i| + |y_i|)^p \right)^{\frac{1}{p}} \leq \left( \sum_{i=1}^n |x_i|^p \right)^{1/p} + \left( \sum_{i=1}^n |y_i|^p \right)^{1/p}$
\end{enumerate}
